\def\restrict{r}
\def\prolongate{p}
\begin{example}
  Smoothing property of the Gauss-Seidel method for the one-dimensional Laplacian.
  \begin{figure}[tp]
    \begin{center}
      \includegraphics[width=.49\textwidth]{../graph/smoothing/gauss-seidel-0.tikz}
      \includegraphics[width=.49\textwidth]{../graph/smoothing/gauss-seidel-3.tikz}
      \includegraphics[width=.49\textwidth]{../graph/smoothing/gauss-seidel-1.tikz}
      \includegraphics[width=.49\textwidth]{../graph/smoothing/gauss-seidel-4.tikz}
      \includegraphics[width=.49\textwidth]{../graph/smoothing/gauss-seidel-2.tikz}
      \hbox to .49\textwidth{}
    \end{center}
    \caption{Development of the error of the Gauss-Seidel iteration. Random initial error and errors after one and two steps (left). Errors after 3, 4, and 5 steps (top right) and after 10, 20, 40, 80, 160, and 320 steps (lower right).}
  \end{figure}
\end{example}
\begin{Algorithm*}{mgm}{The Multigrid iteration MGM($\ell, u_\ell^{k}, b_\ell$)}
  \index{multigrid iteration}
  \begin{enumerate}
  \item Pre-smoothing: let $u_\ell^{k,0} = u_\ell^{k}$ and for
    $i=0,\dots,\nu_1-1$ do
    \begin{gather}
      u_\ell^{k,i+1} = u_\ell^{k,i}
      + \omega\bigl(b_\ell - A_\ell u_\ell^{k,i}\bigr).
    \end{gather}
  \item Coarse grid correction: compute
    $b_{\ell-1} = \restrict(b_\ell - A_\ell u_\ell^{k,\nu_1})$ and
    \begin{enumerate}
    \item If $\ell=1$ solve $A_0 u_0^{\mu} = b_0$ exactly
    \item If $\ell>1$, let $u_{\ell-1}^0 = 0$ and for $i=0,\dots,\mu-1$ do
      \begin{gather*}
        u_{\ell-1}^{i+1} = \text{MGM}(\ell-1, u_{\ell-1}^{i},b_{\ell-1}).
      \end{gather*}
      Then, add
      $u_\ell^{k,\nu_1+1} = u_\ell^{k,\nu_1} + \prolongate u_{\ell-1}^{\mu}$.
    \end{enumerate}
  \item Post-smoothing: for $i=\nu_1+1,\dots,\nu_1+\nu_2$ do
    \begin{gather}
      u_\ell^{k,i+1} = u_\ell^{k,i}
      + \omega\bigl(b_\ell - A_\ell u_\ell^{k,i}\bigr).
    \end{gather}
    and let
    $u_\ell^{k+1}=u_\ell^{k,\nu_1+\nu_2+1}$.
  \end{enumerate}
\end{Algorithm*}

\begin{remark}
  The multigrid method for $\mu=1$ is called the V-cycle, for $\mu=2$
  it is the W-cycle. The generalization where $\mu$ depends on $\ell$,
  typically in the form $2^{L-\ell}$, where $L$ is the finest level,
  is called the variable V-cycle.
\end{remark}

\begin{remark}
  The Richardson method in pre- and post-smoothing can be replaced by
  other relaxation methods like Jacobi, Gauss-Seidel, SOR, or
  SSOR. Even more complex operations may be considered.

  If the smoother, like SOR, is not symmetric, it is possible to apply
  the transpose (backward SOR instead of forward) in post-smoothing to
  obtain a method which is symmetric.
\end{remark}

\begin{Lemma}{mgm-error}
  Let $S_\ell$ be the error propagation operator of the
  smoother. Then, the error propagation operator of a single step of
  the multigrid iteration is defined recursively by
  \begin{gather}
    I - M_\ell = S_\ell^{\nu_2}
    (I-\prolongate M_{\ell-1}^{\mu}\restrict A)
    S_\ell^{\nu_1},
  \end{gather}
  and $M_0 = A^{-1}$.
\end{Lemma}

\begin{proof}
  We prove for $k=0$, which proves for every step and omit the superscript $k$.
  First, observe that for the exact solution $u_\ell$ of
  $A_\ell u_\ell = b_\ell$ there holds
  \begin{gather*}
    u_\ell - u_\ell^{i+1}
    = S \left(u_\ell - u_\ell^{i+1}\right)
    \qquad i=i=0,\dots,\nu_1-1,\nu_1+1,\dots,\nu_1+\nu_2.
  \end{gather*}
  Thus,
  \begin{gather*}
    u_\ell - u_\ell^{\nu_1} = S^{\nu_1}(u_\ell - u_\ell^{0}),
    \qquad
    u_\ell - u_\ell^{\nu_1+\nu_2+1}
    = S^{\nu_2}(u_\ell - u_\ell^{\nu_1+1}),
  \end{gather*}
  We continue by induction. For $\ell=1$, we have
  \begin{gather*}
    u_1-u_1^{\nu_1+1}
    = u_1-u_1^{\nu_1} - \prolongate u_{0}^{\mu}
    = u_1-u_1^{\nu_1} - \prolongate A_0^{-1}
     \restrict A_1(u_1-u_1^{\nu_1}).
   \end{gather*}
   Combining with the error propagation of pre and post smoothing, we
   get
  \begin{gather*}
    u_1 -u_1^{\nu_1+\nu_2+1}
    = S_\ell^{\nu_2}
    (I-\prolongate A_0^{-1} \restrict A_1)
    S_\ell^{\nu_1} \left(u_1 -u_1^{0}\right).
  \end{gather*}
\end{proof}

%%% Local Variables:
%%% mode: latex
%%% TeX-master: "main"
%%% End:
