\begin{Lemma}{lmm-one-step}
  Every multistep method can be recast as a one-step method
  \begin{gather}
    \label{eq:lmm-one-step:1}
    Y_{k} = (A \otimes \identity) Y_{k-1} + h \verfahren_h(t_{k-1}, Y_{k-1})
  \end{gather}
  where with $\alpha_r' = \alpha_r/\alpha_s$
  \begin{gather}
    \label{eq:lmm-one-step:2}
    Y_k =
    \begin{pmatrix}
      y_k \\ \vdots \\ y_{k-s+1}
    \end{pmatrix},
    \quad
    A =
    \begin{pmatrix}
      -\alpha_{\lmms-1}' & -\alpha_{\lmms-2}' & \cdots & -\alpha_{0}'\\
      1 & 0 & \cdots & 0 \\
      & \ddots & \cdots & 0 \\
      & & 1 & 0
    \end{pmatrix},
  \end{gather}
  and $\verfahren_h(t_k, Y_k) = (e_1 \otimes \identity) \psi_h(t_{k-1}, Y_{k-1})$ with
  $\beta_r' = \beta_r/\alpha_s$ and $\psi_h$ defined implicitly by
  \begin{multline}
    \label{eq:lmm-one-step:3}
    \psi_h(t_{k-1}, Y_{k-1})
    =\sum_{r=1}^{\lmms} \beta_{\lmms-r} f(t_{k-r},y_{k-r})
    \\
    + \beta_s' f\left(t_k, h\psi_h(t_{k-1}, Y_{k-1}) -
      \sum_{r=1}^{\lmms} \alpha_{\lmms-r}' y_{k-r}\right).
  \end{multline}
\end{Lemma}

%%% Local Variables: 
%%% mode: latex
%%% TeX-master: "../notes"
%%% End: 
