\section{Derivatives of the solutions of IVP with respect to data}
\subsection{Derivatives with respect to the initial values}
\begin{intro}
  In order to understand BVP, we have to introduce the notion of the
  derivative of the solution to an IVP with respect to its initial
  values. Our interest lies in the change of $u$ if the initial value
  is changed. We will thus denote in these cases $u=u(t;v)$, where $t$ is
  the usual ``time'' variable and $v$ the initial value, which now is
  a variable as well. Thus, $u(t;v)$ is the solution to the IVP
  \begin{gather}
    \label{eq:derivatives:1}
    \begin{split}
      u'(t;v) = \tfrac{\partial}{\partial t} u(t;v) &= f\bigl(t,u(t;v)\bigr) \\
      u(t_0;v) &= v.
    \end{split}
  \end{gather}
  The purpose of this section is the study of the derivative
  \begin{gather*}
    \tfrac{\partial}{\partial v} u(t;v),
  \end{gather*}
  which is fundamentally different from $\nicefrac{\partial}{\partial t}
  u(t;v)$.
  It can be obtained by solving the variational equation of the
  original IVP, defined as follows.
\end{intro}

\begin{Definition}{gateaux-derivative}
  Let $F(v)$ be a function defined on some function space. Then, the G창teaux
  derivative of $F$ at a point $v$ in direction $w$ with $v$ and $w$
  in this function space is defined as
  \begin{gather}
    \label{eq:derivatives:6}
    \frac{\partial}{\partial w} F(v)
    = \lim_{\epsilon\to 0} \frac{F(v+\epsilon w) - F(v)}{\epsilon},
  \end{gather}
  if this limit exists.
  
  Here, we have used the notation for directional derivatives in
  $\R^n$, since this is indeed the character of the G창teaux
  derivative.
  % Let $f$ be a function depending on another function $v$. Then, the
  % \define{Gateaux derivative} of $f$ at $v$ in direction $w$ is
  % defined as
  
\end{Definition}
% \begin{remark}
%   In terms of linear \putindex{perturbation theory} this section deals
%   with the derivative of the solution $u(t)$ of the
%   IVP~\eqref{eq:awa}, but not with respect to the argument $t$, but
%   rather with respect to the initial values. That is why we will write
%   the solution $u = u(t;s)$ of the IVP
%   \begin{gather}
%     \label{eq:derivatives:1}
%     \begin{split}
%       u'(t;s) = \tfrac{\partial}{\partial t} u(t;s) &= f\bigl(t,u(t;s)\bigr) \\
%       u(t_0;s) &= s_0
%     \end{split}
%   \end{gather}
%   with two arguments, the actual time variable $t$ and the initial value $s$.
% \end{remark}

\input{definitions/variational-equation}

\begin{remark}
  The fundamental matrix $\fundam$ can also be read column
  by column.  Then each column is a vector-valued function
  $\phi^{(i)}(t)$ and solves the IVP
  \begin{gather*}
    \begin{split}
      \tfrac{d}{dt}\phi^{(i)}(t) &= \nabla_u
      f\bigl(t,u(t)\bigr)\phi^{(i)}(t),
      \\
      \phi^{(i)}(t_0) &= e_i.
    \end{split}
  \end{gather*}
\end{remark}

\begin{remark}
  The definition of the fundamental matrix here is consistent with the
  one in Definition~\ref{Definition:fundamental-system} for linear
  equations. Namely, for $f(u) = Au$, we have $\nabla_u f(u) = A$.
\end{remark}

\input{theorems/fundamental}

\begin{proof}
  In order to prove the first equation, denote by $V(\tau;s)$ the
  solution to the IVP
  \begin{gather*}
    V'(\tau;s) = \nabla_u f(\tau,u(\tau)) V(\tau;s),
    \qquad V(s;s) = \fundamental(s;t).
  \end{gather*}
  Because of uniqueness, we must have
  $V(\tau;s) = \fundamental(\tau;t)$ for any $\tau$ between $s$ and
  $t$, in particular for $r=t$, such that $V(t;s) = \fundamental(t;t) = \identity$. On the
  other hand, by linearity, we have
  $V(\tau;s) = \fundamental(\tau;s)\fundamental(s;t)$, and thus the
  equation is proven by
  \begin{gather*}
    \identity = V(t;s) = \fundamental(t;s)\fundamental(s;t).
  \end{gather*}

  Now, assume without loss of generality that $s$ is between $r$ and
  $t$. Indeed, if for instance $t$ is between $r$ and $s$, multiply
  equation~\eqref{eq:derivatives:4} from the left by $\fundamental(s;t)$ and
  prove the equation for
  \begin{gather*}
    \fundamental(s;t)\fundamental(t;r)
    = \fundamental(s;t)\fundamental(t;s)U(s;r)
    = \fundamental(s;r).
  \end{gather*}
  Take the auxiliary function $V(\tau;s)$ as defined above. By
  uniqueness, it is equal to $\fundamental(\tau;t)$ for all $\tau$. But, on the
  other hand, we have by linearity $V(\tau;s) = \fundamental(\tau;s)\fundamental(s;r)$, in
  particular for $\tau=t$.

  The statement follows from the definition as a solution of an IVP
  and the fact that solutions of linear IVP are linear combinable.
\end{proof}

\input{theorems/derivative}

\begin{proof}
  We write the IVP in its full dependence on $v$ as
  \begin{align*}
    \frac{\partial u(t;v)}{\partial t} &= f\bigl(t,u(t;v)\bigr) \\
    u(t_0;v) &= v.
  \end{align*}
  From the second equation, we immediately obtain
  \begin{gather*}
    \frac{\partial u(t_0;v)}{\partial v} = \identity.
  \end{gather*}
Assuming differentiability of $f$ with respect to $u$, the first
equation yields
\begin{gather*}
  \frac{\partial}{\partial v}\frac{\partial u(t;v)}{\partial t}
  = \frac{\partial f\bigl(t,u(t;v)\bigr)}{\partial v}
  = \nabla_u f(t,u(t;v)) \frac{\partial u(t;v)}{\partial v}.
\end{gather*}
Thus, $\tfrac{\partial}{\partial v} u$ solves the
IVP~\eqref{eq:derivatives:1}
\begin{gather*}
  \left( \frac{\partial}{\partial v} u \right)'
  = \nabla_u f(t,u(t;v)) \frac{\partial u(t;v)}{\partial v}.
\end{gather*}
$\tfrac{\partial}{\partial v} u$ solves the same IVP as the
fundamental matrix and thus, they coincide.
\end{proof}

\subsection{Derivatives with respect to the right hand side function}
\begin{intro}
  We close this section by studying the differential dependence of the
  solution $u(t)$ of an ODE at time $t$ on the function $f(t,u)$, that
  is, the derivative of a value with respect to a function. In order
  to keep things simple, we reduce this question to a regular
  derivative of a function with respect to a real variable by using
  the G창teaux derivative.
  Back to differential equations, our task is now to compute the
  derivative of $u(t)$ with respect to changes in $f$, denoted as
  \begin{gather}
    \label{eq:derivatives:7}
    \frac{\partial}{\partial g} u(t)
    = \lim_{\epsilon\to 0} \frac{u_\epsilon-u}{\epsilon}
    = \left.\frac{d}{d\epsilon} u_\epsilon(t)\right|_{\epsilon=0},
  \end{gather}
  where $u$ and $u_\epsilon$ respectively solve the IVPs
  \begin{xalignat*}{2}
    u'&=f(t,u) & u(t_0)& = u_0 \\
    u_\epsilon'&=f(t,u_\epsilon)+\epsilon g(t,u_\epsilon)
    & u_\epsilon(t_0)& = u_0.
  \end{xalignat*}
  For this derivative, we have the following theorem.
\end{intro}

\input{theorems/derivative-f.tex}

\begin{proof}
   We set out by devising a differential equation for the G창teaux
  derivative $\mathcal U(t) := \left.\frac{d}{d\epsilon} u_\epsilon(t)\right|_{\epsilon=0}$. The differential equation for $u$ yields
  \begin{align*}
    \mathcal U'(t) =& \left( \left.\frac{d}{d\epsilon} u_\epsilon(t)\right|_{\epsilon=0} \right)' \\
    =& \left.\frac{d}{d\epsilon} u_\epsilon ' (t)\right|_{\epsilon=0} \\
    =& \left.\frac{d}{d\epsilon}
    \Bigl(f\bigl(t,u_\epsilon(t)\bigr)
    + \epsilon g\bigl(t,u_\epsilon(t)\bigr)\Bigr) \right|_{\epsilon=0} \\
    =& \left.\nabla_u f(t,u_\epsilon) \frac{d}{d\epsilon} u_\epsilon(t)
     + \epsilon \nabla_u g \bigl(u_\epsilon (t) \bigr) \frac{d}{d\epsilon} u_\epsilon(t) 
    + g\bigl(t,u_\epsilon(t)\bigr) \right|_{\epsilon=0}
  \\
    =& \left.\nabla_u f(t,u_\epsilon) \mathcal U(t)
    + g\bigl(t,u_\epsilon(t)\bigr) \right|_{\epsilon=0}
  \end{align*}
  Furthermore, we have
  \begin{gather*}
     \mathcal U(t_0) = \frac{d}{d\epsilon} u_\epsilon(t_0) = 0.
  \end{gather*}

  According to Lemma~\ref{Lemma:linear-representation}, the solution
  of this initial value problem can be represented with the
  integrating factor $M(t)$ as
  \begin{gather*}
    \mathcal U(t) = M^{-1}(t) \int_{t_0}^t M(s) g\bigl(s,u(s)\bigr)
    \, \ds.
  \end{gather*}
  Noticing that $M(\tau)^{-1} = \fundamental(\tau;t_0)$, we obtain
  \begin{gather*}
    u(t) = \int_{t_0}^t \fundamental(t;s) g\bigl(s,u(s)\bigr) \, \ds
\end{gather*}
\end{proof}


%%% Local Variables: 
%%% mode: latex
%%% TeX-master: "notes"
%%% End: 
